Nearing the proof of cancellation

formal-proofs/theories/lib/infinite_array/infinite_array_impl.v
@@ -242,11 +242,6 @@ Definition ias_cell_info' (id_seg id_cell: nat) (c: cell_algebra):
   listUR segment_algebra :=
   ias_segment_info id_seg (ε, replicate id_cell ε ++ [c]).
 
-Definition ias_cell_info (id: nat) (c: cell_algebra): listUR segment_algebra :=
-  let ns := (id `div` Pos.to_nat segment_size)%nat in
-  let nc := (id `mod` Pos.to_nat segment_size)%nat in
-  ias_cell_info' ns nc c.
-
 Theorem ias_cell_info'_op ns nc s s':
   ias_cell_info' ns nc (s ⋅ s') =
   ias_cell_info' ns nc s ⋅ ias_cell_info' ns nc s'.
@@ -291,14 +286,18 @@ Proof.
     induction nc; case; done.
 Qed.
 
-Theorem ias_cell_info__ias_cell_info' ns nc n s:
+Definition ias_cell_info_view {A: Type} f id: A :=
+  let ns := (id `div` Pos.to_nat segment_size)%nat in
+  let nc := (id `mod` Pos.to_nat segment_size)%nat in
+  f ns nc.
+
+Theorem ias_cell_info_view_eq {A: Type} ns nc n (f: nat -> nat -> A):
   (nc < Pos.to_nat segment_size)%nat ->
   n = (nc + ns * Pos.to_nat segment_size)%nat ->
-  ias_cell_info' ns nc s = ias_cell_info n s.
+  f ns nc = ias_cell_info_view f n.
 Proof.
-  rewrite /ias_cell_info /ias_cell_info'.
-  intros Hlt Heq.
-  subst.
+  rewrite /ias_cell_info_view.
+  intros Hlt Heq. subst.
   replace ((nc + ns * Pos.to_nat segment_size) `div` Pos.to_nat segment_size)%nat
     with ns.
   replace ((nc + ns * Pos.to_nat segment_size) `mod` Pos.to_nat segment_size)%nat
@@ -335,9 +334,7 @@ Proof.
 Qed.
 
 Definition array_mapsto γ (id: nat) (ℓ: loc): iProp :=
-  let ns := (id `div` Pos.to_nat segment_size)%nat in
-  let nc := (id `mod` Pos.to_nat segment_size)%nat in
-  array_mapsto' γ ns nc ℓ.
+  ias_cell_info_view (fun ns nc => array_mapsto' γ ns nc ℓ) id.
 
 Theorem array_mapsto'_agree γ (ns nc: nat) (ℓ ℓ': loc):
   array_mapsto' γ ns nc ℓ -∗ array_mapsto' γ ns nc ℓ' -∗ ⌜ℓ = ℓ'⌝.
@@ -363,7 +360,7 @@ Theorem array_mapsto_agree γ n (ℓ ℓ': loc):
   array_mapsto γ n ℓ -∗ array_mapsto γ n ℓ' -∗ ⌜ℓ = ℓ'⌝.
 Proof. apply array_mapsto'_agree. Qed.
 
-Global Instance array_mapsto_persistent γ n ℓ: Persistent (array_mapsto γ n ℓ).
+Global Instance array_mapsto_persistent γ ns nc ℓ: Persistent (array_mapsto' γ ns nc ℓ).
 Proof. apply _. Qed.
 
 End array_mapsto.
@@ -377,14 +374,15 @@ Global Instance segment_is_cancelled_persistent γ n:
   Persistent (segment_is_cancelled γ n).
 Proof. by segment_info_persistent. Qed.
 
-Definition cell_is_cancelled γ (n: nat): iProp :=
-  own γ (◯ (ias_cell_info n (Some (Cinl (to_agree tt))))).
+Definition cell_is_cancelled' γ (ns nc: nat): iProp :=
+  own γ (◯ (ias_cell_info' ns nc (Some (Cinl (to_agree tt))))).
+Definition cell_is_cancelled γ := ias_cell_info_view (cell_is_cancelled' γ).
 
-Definition cell_cancellation_handle γ (id: nat): iProp :=
-  own γ (◯ (ias_cell_info id (Some (Cinr (3/4)%Qp)))).
+Definition cell_cancellation_handle' γ (ns nc: nat): iProp :=
+  own γ (◯ (ias_cell_info' ns nc (Some (Cinr (3/4)%Qp)))).
 
-Theorem cell_cancellation_handle_exclusive γ (id: nat):
-  cell_cancellation_handle γ id -∗ cell_cancellation_handle γ id -∗ False.
+Theorem cell_cancellation_handle'_exclusive γ (ns nc: nat):
+  cell_cancellation_handle' γ ns nc -∗ cell_cancellation_handle' γ ns nc -∗ False.
 Proof.
   iIntros "HCh1 HCh2".
   iDestruct (own_valid_2 with "HCh1 HCh2") as %HContra.
@@ -726,8 +724,7 @@ Proof.
   iDestruct (segment_canc_location_agree with "HIsCancLoc HCancLoc") as %->.
   wp_load.
   iMod ("HClose" $! cancelled with "[HCanc Hℓ Hpℓ Hcℓ Hnℓ]") as "HΦ".
-  { iDestruct "HCanc" as (cells) "[% [#HCancelled HCanc]]".
-    subst.
+  { iDestruct "HCanc" as (cells) "[-> [#HCancelled HCanc]]".
     iSplitL.
     { rewrite /is_segment /is_segment'; eauto 20 with iFrame. }
     iExists cells. iSplit; done.
@@ -735,6 +732,169 @@ Proof.
   iModIntro.
   by wp_pures.
 Qed.
+
+Theorem list_lookup_local_update {A: ucmraT}:
+  forall (x y x' y': list A),
+    (forall i, (x !! i, y !! i) ~l~> (x' !! i, y' !! i)) ->
+    (x, y) ~l~> (x', y').
+Proof.
+  intros x y x' y' Hup.
+  apply local_update_unital=> n z Hxv Hx.
+  unfold local_update in Hup.
+  simpl in *.
+  assert (forall i, ✓{n} (x' !! i) /\ x' !! i ≡{n}≡ (y' ⋅ z) !! i) as Hup'.
+  { intros i. destruct (Hup i n (Some (z !! i))); simpl in *.
+    - by apply list_lookup_validN.
+    - rewrite -list_lookup_op.
+      by apply list_dist_lookup.
+    - rewrite list_lookup_op. split; done.
+  }
+  split; [apply list_lookup_validN | apply list_dist_lookup].
+  all: intros i; by destruct (Hup' i).
+Qed.
+
+Theorem list_append_local_update {A: ucmraT}:
+  forall (x z: list A), (forall n, ✓{n} z) -> (x, ε) ~l~> (x ++ z, (replicate (length x) ε) ++ z).
+Proof.
+  intros ? ? Hzv. apply local_update_unital=> n mz Hxv Hx.
+  split; first by apply Forall_app_2; [apply Hxv|apply Hzv].
+  rewrite Hx.
+  replace (ε ⋅ mz) with mz by auto.
+  rewrite list_op_app_le.
+  2: by rewrite replicate_length.
+  assert (replicate (length mz) ε ⋅ mz ≡ mz) as Heq.
+  { clear. apply list_equiv_lookup.
+    induction mz; simpl; first done.
+    destruct i; simpl.
+    by rewrite ucmra_unit_left_id.
+    done.
+  }
+  by rewrite Heq.
+Qed.
+
+Theorem list_alter_local_update {A: ucmraT}:
+  forall n f g (x y: list A),
+    (x !! n, y !! n) ~l~> (f <$> (x !! n), g <$> (y !! n)) ->
+    (x, y) ~l~> (list_alter f n x, list_alter g n y).
+Proof.
+  intros ? ? ? ? ? Hup.
+  apply list_lookup_local_update.
+  intros i.
+  destruct (nat_eq_dec i n); subst.
+  - by repeat rewrite list_lookup_alter.
+  - by repeat rewrite list_lookup_alter_ne.
+Qed.
+
+Lemma None_local_update {A: cmraT}: forall (x: A) a b, (None, Some x) ~l~> (a, b).
+Proof.
+  intros ? ? ? n mz _ Heq. exfalso. simpl in *.
+  symmetry in Heq. apply (dist_None n _) in Heq.
+  destruct mz; simpl in Heq.
+  1: rewrite Some_op_opM in Heq.
+  all: discriminate.
+Qed.
+
+Check option_included.
+
+Theorem segment_canc_incr_spec γ id cid (ℓ cℓ: loc) segments:
+  (cid < Pos.to_nat segment_size)%nat ->
+  <<< ∀ pl nl, is_segment γ id ℓ pl nl ∗ segment_canc_location γ id cℓ ∗
+                              cell_cancellation_handle' γ id cid ∗
+                              own γ (● segments) >>>
+    FAA #cℓ #1 @ ⊤
+  <<< ∃ (cancelled: nat),
+        is_segment γ id ℓ pl nl ∗
+    (∃ cells,
+          cancelled_cells γ id cells
+                          ∗ ⌜cancelled = length (List.filter (fun i => i) (vec_to_list cells))⌝) ∗
+    (∃ segments', own γ (● segments')),
+    RET #cancelled >>>.
+Proof.
+  iIntros (HCid Φ) "AU".
+  iMod "AU" as (pl nl) "[[HIsSeg [#HIsCancLoc [HCancHandle HAuth]]] [_ HClose]]".
+  rename cℓ into cℓ'. iDestructHIsSeg.
+  iDestruct (segment_canc_location_agree with "HIsCancLoc HCancLoc") as %->.
+  iDestruct "HCanc" as (cells) "[-> [#HCancelled HCanc]]".
+  rewrite /cell_cancellation_handle' /ias_cell_info'.
+  iCombine "HCanc" "HCancHandle" as "HSeg".
+  rewrite -ias_segment_info_op.
+  rewrite pair_op.
+  iMod (own_update_2 with "HAuth HSeg") as "[HAuth HSeg]".
+  { apply auth_update.
+    apply (let update_list := list_alter (fun _ => Some (Cinl (to_agree ()))) cid in
+           let auth_fn x := ((x.1.1, (fun i => i) <$> x.1.2), update_list x.2) in
+           let frag_fn x := ((x.1.1, (fun i => i) <$> x.1.2), update_list x.2)
+           in list_alter_local_update id auth_fn frag_fn).
+    rewrite ias_segment_info_lookup.
+    simpl.
+    unfold lookup.
+    destruct (list_lookup id segments); simpl.
+    2: by apply None_local_update.
+    repeat rewrite ucmra_unit_right_id.
+    apply option_local_update.
+    apply prod_local_update; simpl.
+    apply prod_local_update_2; simpl.
+    {
+      destruct u as [[ULocs [UCanc|]] UCells]; simpl.
+      2: by apply None_local_update.
+      apply option_local_update.
+      admit.
+    }
+    {
+      apply list_alter_local_update.
+      repeat rewrite list_lookup_op.
+      rewrite lookup_app_r replicate_length. rewrite -minus_diag_reverse; simpl.
+      2: lia.
+      remember (map _ _) as lst'.
+      assert (is_Some (list_lookup cid lst')) as [x Hcell].
+      { apply lookup_lt_is_Some. subst.
+        rewrite map_length. rewrite vec_to_list_length.
+        done.
+      }
+      unfold lookup.
+      rewrite Hcell.
+      subst lst'.
+      apply list_lookup_fmap_inv in Hcell.
+      destruct Hcell as [was_cancelled [-> Hcellid]].
+      repeat rewrite -Some_op.
+      destruct was_cancelled.
+      { rewrite /op /cmra_op /=.
+        intros n mz Hxv Heq.
+        move: Hxv. rewrite Heq.
+        simpl.
+        destruct mz; simpl.
+        destruct c.
+        destruct c.
+        all: done.
+      }
+      simpl.
+      rewrite Cinr_op.
+      apply local_update_total_valid.
+      remember (list_lookup _ _) as He.
+      intros HeValid _ HeEq.
+      assert (forall (A: ucmraT) (a b: A), a ≡ b ∨ a ≼ b -> a ≼ b) as HSimpl.
+      { clear. intros. destruct H; auto. unfold included. exists ε.
+        rewrite ucmra_unit_right_id. auto. }
+      apply option_included in HeEq.
+      destruct HeEq as [?|[a [b [Heq1 [Heq2 HeEq]]]]]; subst; first discriminate.
+      rewrite Heq2; simpl.
+      apply option_local_update.
+      apply transitivity with (y := (None, None)).
+      { apply delete_option_local_update.
+        apply Cinr_exclusive.
+        replace ((1/4) ⋅ (3/4))%Qp with 1%Qp.
+        1: by apply frac_full_exclusive.
+        symmetry.
+        apply Qp_quarter_three_quarter.
+      }
+      apply alloc_option_local_update.
+      done.
+    }
+  }
+  wp_faa.
+  iMod ("HClose" $! (length (List.filter (fun i => i) (vec_to_list cells)))%nat with "[Hℓ Hpℓ Hcℓ Hnℓ HAuth]") as "HΦ".
+  2: by iModIntro.
+Abort.
 
 Theorem segment_data_at_spec γ id (ℓ: loc) (ix: nat):
   ⌜ix < Pos.to_nat segment_size⌝ -∗
